Bhaktish/validator soundness (#2)
complete proof of the soundness of the cedar validator

cedar-lean/Cedar/Thm/Validation/Validator.lean
@@ -1,3 +1,19 @@
+/-
+ Copyright 2022-2023 Amazon.com, Inc. or its affiliates. All Rights Reserved.
+
+ Licensed under the Apache License, Version 2.0 (the "License");
+ you may not use this file except in compliance with the License.
+ You may obtain a copy of the License at
+
+      https://www.apache.org/licenses/LICENSE-2.0
+
+ Unless required by applicable law or agreed to in writing, software
+ distributed under the License is distributed on an "AS IS" BASIS,
+ WITHOUT WARRANTIES OR CONDITIONS OF ANY KIND, either express or implied.
+ See the License for the specific language governing permissions and
+ limitations under the License.
+-/
+
 import Cedar.Spec
 import Cedar.Data
 import Cedar.Validation
@@ -10,227 +26,376 @@ open Cedar.Data
 open Cedar.Spec
 open Cedar.Validation
 
--- for a single expression, evaluates to a boolean value (or appropriate error)
+/-- for a single expression, evaluates to a boolean value (or appropriate error) -/
 def OneEvaluatesCorrectly (expr : Expr) (request : Request) (entities : Entities) : Prop :=
-∃ (b : Bool), EvaluatesTo expr request entities b
+  ∃ (b : Bool), EvaluatesTo expr request entities b
 
--- every policy as an expression evaluates to a boolean value or appropriate error
+/-- every policy as an expression evaluates to a boolean value or appropriate error -/
 def AllEvaluateCorrectly (policies : Policies) (request : Request) (entities : Entities) : Prop :=
-∀ policy : Policy, policy ∈ policies → OneEvaluatesCorrectly policy.toExpr request entities
+  ∀ policy : Policy, policy ∈ policies → OneEvaluatesCorrectly policy.toExpr request entities
+
+def RequestAndEntitiesMatchSchema (schema : Schema) (request : Request) (entities : Entities) :Prop :=
+  ∀ env ∈ schema.toEnvironments,
+  RequestAndEntitiesMatchEnvironment env request entities
 
 def EvaluatesSubst (expr : Expr) (request : Request) (entities : Entities) : Prop :=
-evaluate (substituteAction request.action expr) request entities = evaluate expr request entities
+  evaluate (substituteAction request.action expr) request entities = evaluate expr request entities
+
 
 theorem evaluates_subst_ite {i t e : Expr} {request : Request} {entities : Entities}
 (ih₁ : EvaluatesSubst i request entities)
 (ih₂ : EvaluatesSubst t request entities)
 (ih₃ : EvaluatesSubst e request entities) :
-evaluate (substituteAction request.action (Expr.ite i t e)) request entities =
-evaluate (Expr.ite i t e) request entities := by
-simp [EvaluatesSubst, substituteAction, mapOnVars] at *
-simp [evaluate, ih₁, ih₂, ih₃]
+  evaluate (substituteAction request.action (Expr.ite i t e)) request entities =
+  evaluate (Expr.ite i t e) request entities
+:= by
+  simp only [EvaluatesSubst, substituteAction, mapOnVars] at *
+  simp only [evaluate, ih₁, ih₂, ih₃]
 
 theorem evaluates_subst_getAttr {e : Expr} {attr : Attr} {request : Request} {entities : Entities}
 (ih₁ : EvaluatesSubst e request entities) :
-evaluate (substituteAction request.action (Expr.getAttr e attr)) request entities =
-evaluate (Expr.getAttr e attr) request entities := by
-simp [EvaluatesSubst] at ih₁
-simp [substituteAction, mapOnVars] at *
-simp [evaluate, ih₁]
+  evaluate (substituteAction request.action (Expr.getAttr e attr)) request entities =
+  evaluate (Expr.getAttr e attr) request entities
+:= by
+  simp only [EvaluatesSubst] at ih₁
+  simp only [substituteAction, mapOnVars] at *
+  simp only [evaluate, ih₁]
 
 theorem evaluates_subst_hasAttr {e : Expr} {attr : Attr} {request : Request} {entities : Entities}
 (ih₁ : EvaluatesSubst e request entities) :
-evaluate (substituteAction request.action (Expr.hasAttr e attr)) request entities =
-evaluate (Expr.hasAttr e attr) request entities := by
-simp [EvaluatesSubst] at ih₁
-simp [substituteAction, mapOnVars] at *
-simp [evaluate, ih₁]
+  evaluate (substituteAction request.action (Expr.hasAttr e attr)) request entities =
+  evaluate (Expr.hasAttr e attr) request entities
+:= by
+  simp only [EvaluatesSubst] at ih₁
+  simp only [substituteAction, mapOnVars] at *
+  simp only [evaluate, ih₁]
 
 theorem evaluates_subst_unaryApp {op : UnaryOp} {e : Expr} {request : Request} {entities : Entities}
 (ih₁ : EvaluatesSubst e request entities) :
-evaluate (substituteAction request.action (Expr.unaryApp op e)) request entities =
-evaluate (Expr.unaryApp op e) request entities := by
-simp [EvaluatesSubst] at ih₁
-simp [substituteAction, mapOnVars] at *
-simp [evaluate, ih₁]
+  evaluate (substituteAction request.action (Expr.unaryApp op e)) request entities =
+  evaluate (Expr.unaryApp op e) request entities
+:= by
+  simp only [EvaluatesSubst] at ih₁
+  simp only [substituteAction, mapOnVars] at *
+  simp only [evaluate, ih₁]
 
 theorem evaluates_subst_binaryApp {op : BinaryOp} {a b : Expr} {request : Request} {entities : Entities}
 (ih₁ : EvaluatesSubst a request entities)
 (ih₂ : EvaluatesSubst b request entities) :
-evaluate (substituteAction request.action (Expr.binaryApp op a b)) request entities =
-evaluate (Expr.binaryApp op a b) request entities := by
-simp [EvaluatesSubst] at *
-simp [substituteAction, mapOnVars] at *
-simp [evaluate, ih₁, ih₂]
+  evaluate (substituteAction request.action (Expr.binaryApp op a b)) request entities =
+  evaluate (Expr.binaryApp op a b) request entities
+:= by
+  simp only [EvaluatesSubst] at *
+  simp only [substituteAction, mapOnVars] at *
+  simp only [evaluate, ih₁, ih₂]
 
 theorem evaluates_subst_and {a b : Expr} {request : Request} {entities : Entities}
 (ih₁ : EvaluatesSubst a request entities)
 (ih₂ : EvaluatesSubst b request entities) :
-evaluate (substituteAction request.action (Expr.and a b)) request entities =
-evaluate (Expr.and a b) request entities := by
-simp [EvaluatesSubst, substituteAction, mapOnVars] at *
-simp [evaluate, ih₁, ih₂]
+  evaluate (substituteAction request.action (Expr.and a b)) request entities =
+  evaluate (Expr.and a b) request entities
+:= by
+  simp only [EvaluatesSubst, substituteAction, mapOnVars] at *
+  simp only [evaluate, ih₁, ih₂]
 
 theorem evaluates_subst_or {a b : Expr} {request : Request} {entities : Entities}
 (ih₁ : EvaluatesSubst a request entities)
 (ih₂ : EvaluatesSubst b request entities) :
-evaluate (substituteAction request.action (Expr.or a b)) request entities =
-evaluate (Expr.or a b) request entities := by
-simp [EvaluatesSubst, substituteAction, mapOnVars] at *
-simp [evaluate, ih₁, ih₂]
+  evaluate (substituteAction request.action (Expr.or a b)) request entities =
+  evaluate (Expr.or a b) request entities
+:= by
+  simp only [EvaluatesSubst, substituteAction, mapOnVars] at *
+  simp only [evaluate, ih₁, ih₂]
+
+theorem substitute_action_nil_set : ∀ (uid : EntityUID),
+  substituteAction uid (.set []) = .set []
+:= by
+  intro uid
+  simp only [substituteAction, mapOnVars, List.attach_def, List.pmap, List.map_nil]
+
+theorem substitute_action_cons_set : ∀ (h : Expr) (t : List Expr) (uid : EntityUID),
+  substituteAction uid (.set (h :: t)) = .set ((substituteAction uid h) :: t.map (substituteAction uid))
+:= by
+  intro h t uid
+  simp only [substituteAction, mapOnVars, List.attach_def, List.map_pmap_subtype, List.map_cons]
+  simp only [Expr.set.injEq, List.cons.injEq, true_and]
+  unfold substituteAction
+  simp only
+
+theorem forall_map {xs : List Expr} {f g : Expr → Result Value}
+(h₀ : ∀ x ∈ xs, f x = g x) :
+  List.mapM f xs = List.mapM g xs
+:= by
+  induction xs
+  case nil =>
+    simp only [List.mapM_nil]
+  case cons h t ih =>
+    simp only [List.mapM_cons]
+    simp [List.mem_cons] at h₀
+    obtain ⟨h₁, h₂⟩ := h₀
+    rw [h₁, ih]
+    assumption
 
 theorem evaluates_subst_set {xs : List Expr} {request : Request} {entities : Entities}
 (ih₁ : ∀ xᵢ, xᵢ ∈ xs → EvaluatesSubst xᵢ request entities) :
-evaluate (substituteAction request.action (Expr.set xs)) request entities =
-evaluate (Expr.set xs) request entities := by
-simp [EvaluatesSubst] at ih₁
-sorry
+  evaluate (substituteAction request.action (Expr.set xs)) request entities =
+  evaluate (Expr.set xs) request entities
+:= by
+  cases h₀ : xs with
+  | nil =>
+    rw [substitute_action_nil_set]
+  | cons h t =>
+    simp only [EvaluatesSubst] at ih₁
+    have h₁ := ih₁ h
+    simp only [h₀, List.mem_cons, true_or, true_implies] at h₁
+    rw [substitute_action_cons_set]
+    simp only [mapOnVars, evaluate, List.mapM₁, List.attach_def, List.mapM_pmap_subtype (fun x => evaluate x request entities)]
+    simp only [List.mapM_cons, bind_assoc, pure_bind]
+    rw [h₁]
+    simp [List.mapM_map]
+    have h₂ : ∀ (x₁ : Expr), x₁ ∈ t → EvaluatesSubst x₁ request entities :=
+    by
+      simp [h₀] at ih₁
+      obtain ⟨_, h₂⟩ := ih₁
+      exact h₂
+    rw [forall_map h₂]
+
+theorem substitute_action_nil_record : ∀ (uid : EntityUID),
+  substituteAction uid (.record []) = .record []
+:= by
+  intro uid
+  simp only [substituteAction, mapOnVars, List.attach₂, List.pmap, List.map_nil]
+
+theorem substitute_action_cons_record : ∀ (h : Attr × Expr) (t : List (Attr × Expr)) (uid : EntityUID),
+  substituteAction uid (.record (h :: t)) =
+  .record ((h.fst, substituteAction uid h.snd) :: t.map (fun (a, e) => (a, substituteAction uid e)))
+:= by
+  intro h t uid
+  simp only [substituteAction, mapOnVars, List.attach₂, List.map_pmap_subtype_snd, List.map_cons]
+
+theorem forall_map_record {t : List (Attr × Expr)} {f g : (Attr × Expr) → Result (Attr × Value)}
+(h₀ : ∀ x₁ ∈ t, f x₁ = g x₁) :
+  List.mapM (fun x => f x) t = List.mapM (fun x => g x) t
+:= by
+  induction t
+  case nil =>
+    simp only [List.mapM_nil]
+  case cons h tl ih =>
+    simp only [List.mapM_cons]
+    simp [List.mem_cons] at h₀
+    obtain ⟨h₁, h₂⟩ := h₀
+    rw [h₁, ih]
+    assumption
 
 theorem evaluates_subst_record {axs : List (Attr × Expr)} {request : Request} {entities : Entities}
 (ih₁ : ∀ axᵢ, axᵢ ∈ axs → EvaluatesSubst axᵢ.snd request entities) :
-evaluate (substituteAction request.action (Expr.record axs)) request entities =
-evaluate (Expr.record axs) request entities := by
-simp [EvaluatesSubst] at ih₁
-sorry
+  evaluate (substituteAction request.action (Expr.record axs)) request entities =
+  evaluate (Expr.record axs) request entities
+:= by
+  cases h₀ : axs with
+  | nil =>
+    rw [substitute_action_nil_record]
+  | cons h t =>
+    simp only [EvaluatesSubst] at ih₁
+    have h₁ := ih₁ h
+    simp only [h₀, List.mem_cons, true_or, true_implies] at h₁
+    rw [substitute_action_cons_record]
+    simp only [mapOnVars, evaluate, List.mapM₂, List.attach₂, List.mapM_pmap_subtype (fun (a, e) => bindAttr a (evaluate e request entities))]
+    simp only [bindAttr]
+    simp only [List.mapM_cons, bind_assoc, Except.bind_ok, pure_bind]
+    rw [h₁]
+    simp only [List.mapM_map]
+    have h₂ : ∀ x ∈ t,
+    (do
+      let v ← evaluate (substituteAction request.action x.snd) request entities
+      Except.ok (x.fst, v)) =
+    (do
+      let v ← evaluate x.snd request entities
+      Except.ok (x.fst, v))
+    := by
+      intro x xin
+      simp [h₀] at ih₁
+      obtain ⟨_, h₂⟩ := ih₁
+      simp [h₂ x xin]
+    rw [forall_map_record h₂]
+
+theorem substitute_action_nil_call : ∀ (uid : EntityUID) (xfn : ExtFun),
+  substituteAction uid (.call xfn []) = .call xfn [] :=
+by
+  intro uid
+  simp only [substituteAction, mapOnVars, List.attach_def, List.pmap, List.map_nil, implies_true]
+
+
+theorem substitute_action_cons_call : ∀ (h : Expr) (t : List Expr) (uid : EntityUID) (xfn : ExtFun),
+  substituteAction uid (.call xfn (h :: t)) = .call xfn ((substituteAction uid h) :: t.map (substituteAction uid)) :=
+by
+  intro h t uid
+  simp only [substituteAction, mapOnVars, List.attach_def, List.map_pmap_subtype, List.map_cons]
+  simp only [Expr.call.injEq, List.cons.injEq, true_and, forall_const]
+  unfold substituteAction
+  simp only
+
 
 theorem evaluates_subst_call {xfn : ExtFun} {xs : List Expr} {request : Request} {entities : Entities}
 (ih₁ : ∀ xᵢ, xᵢ ∈ xs → EvaluatesSubst xᵢ request entities) :
-evaluate (substituteAction request.action (Expr.call xfn xs)) request entities =
-evaluate (Expr.call xfn xs) request entities := by
-simp [EvaluatesSubst] at ih₁
-sorry
+  evaluate (substituteAction request.action (Expr.call xfn xs)) request entities =
+  evaluate (Expr.call xfn xs) request entities
+:= by
+  cases h₀ : xs with
+  | nil =>
+    rw [substitute_action_nil_call]
+  | cons h t =>
+    simp only [EvaluatesSubst] at ih₁
+    have h₁ := ih₁ h
+    simp only [h₀, List.mem_cons, true_or, true_implies] at h₁
+    rw [substitute_action_cons_call]
+    simp only [mapOnVars, evaluate, List.mapM₁, List.attach_def, List.mapM_pmap_subtype (fun x => evaluate x request entities)]
+    simp only [List.mapM_cons, bind_assoc, pure_bind]
+    rw [h₁]
+    simp [List.mapM_map]
+    have h₂ : ∀ (x₁ : Expr), x₁ ∈ t → EvaluatesSubst x₁ request entities :=
+    by
+      simp [h₀] at ih₁
+      obtain ⟨_, h₂⟩ := ih₁
+      exact h₂
+    rw [forall_map h₂]
 
 theorem evaluates_subst (expr : Expr) (request : Request) (entities : Entities) :
-evaluate (substituteAction request.action expr) request entities =
-evaluate expr request entities := by
-cases h₀ : expr with
-| lit p => simp [substituteAction, mapOnVars]
-| var vr =>
-  cases h₁ : vr <;> simp [substituteAction, mapOnVars] <;> try assumption
-  case action => sorry
-| ite i t e =>
-  have ih₁ := evaluates_subst i request entities
-  have ih₂ := evaluates_subst t request entities
-  have ih₃ := evaluates_subst e request entities
-  exact @evaluates_subst_ite i t e request entities ih₁ ih₂ ih₃
-| and a b =>
-  have ih₁ := evaluates_subst a request entities
-  have ih₂ := evaluates_subst b request entities
-  exact @evaluates_subst_and a b request entities ih₁ ih₂
-| or a b =>
-  have ih₁ := evaluates_subst a request entities
-  have ih₂ := evaluates_subst b request entities
-  exact @evaluates_subst_or a b request entities ih₁ ih₂
-| unaryApp op e =>
-  have ih₁ := evaluates_subst e request entities
-  exact @evaluates_subst_unaryApp op e request entities ih₁
-| binaryApp op a b =>
-  have ih₁ := evaluates_subst a request entities
-  have ih₂:= evaluates_subst b request entities
-  exact @evaluates_subst_binaryApp op a b request entities ih₁ ih₂
-| getAttr x attr =>
-  have ih₁ := evaluates_subst x request entities
-  exact @evaluates_subst_getAttr x attr request entities ih₁
-| hasAttr x attr =>
-  have ih₁ := evaluates_subst x request entities
-  exact @evaluates_subst_hasAttr x attr request entities ih₁
-| set xs =>
-  have ih : ∀ xᵢ, xᵢ ∈ xs → EvaluatesSubst xᵢ request entities := by
-    intro xᵢ _
-    exact @evaluates_subst xᵢ request entities
-  exact @evaluates_subst_set xs request entities ih
-| record axs =>
-  have ih : ∀ axᵢ, axᵢ ∈ axs → EvaluatesSubst axᵢ.snd request entities := by
-    intro axᵢ hᵢ
-    have _ : sizeOf axᵢ.snd < 1 + sizeOf axs := by
-      apply List.sizeOf_snd_lt_sizeOf_list hᵢ
-    exact @evaluates_subst axᵢ.snd request entities
-  exact @evaluates_subst_record axs request entities ih
-| call xfn xs =>
-  have ih : ∀ xᵢ, xᵢ ∈ xs → EvaluatesSubst xᵢ request entities := by
-    intro xᵢ _
-    exact @evaluates_subst xᵢ request entities
-  exact @evaluates_subst_call xfn xs request entities ih
+  evaluate (substituteAction request.action expr) request entities =
+  evaluate expr request entities
+:= by
+  cases h₀ : expr with
+  | lit p => simp only [substituteAction, mapOnVars]
+  | var vr =>
+    cases vr <;> simp only [substituteAction, mapOnVars] <;> try assumption
+    case action =>
+      simp [evaluate]
+  | ite i t e =>
+    have ih₁ := evaluates_subst i request entities
+    have ih₂ := evaluates_subst t request entities
+    have ih₃ := evaluates_subst e request entities
+    exact @evaluates_subst_ite i t e request entities ih₁ ih₂ ih₃
+  | and a b =>
+    have ih₁ := evaluates_subst a request entities
+    have ih₂ := evaluates_subst b request entities
+    exact @evaluates_subst_and a b request entities ih₁ ih₂
+  | or a b =>
+    have ih₁ := evaluates_subst a request entities
+    have ih₂ := evaluates_subst b request entities
+    exact @evaluates_subst_or a b request entities ih₁ ih₂
+  | unaryApp op e =>
+    have ih₁ := evaluates_subst e request entities
+    exact @evaluates_subst_unaryApp op e request entities ih₁
+  | binaryApp op a b =>
+    have ih₁ := evaluates_subst a request entities
+    have ih₂:= evaluates_subst b request entities
+    exact @evaluates_subst_binaryApp op a b request entities ih₁ ih₂
+  | getAttr x attr =>
+    have ih₁ := evaluates_subst x request entities
+    exact @evaluates_subst_getAttr x attr request entities ih₁
+  | hasAttr x attr =>
+    have ih₁ := evaluates_subst x request entities
+    exact @evaluates_subst_hasAttr x attr request entities ih₁
+  | set xs =>
+    have ih : ∀ xᵢ, xᵢ ∈ xs → EvaluatesSubst xᵢ request entities := by
+      intro xᵢ _
+      exact @evaluates_subst xᵢ request entities
+    exact @evaluates_subst_set xs request entities ih
+  | record axs =>
+    have ih : ∀ axᵢ, axᵢ ∈ axs → EvaluatesSubst axᵢ.snd request entities := by
+      intro axᵢ hᵢ
+      have _ : sizeOf axᵢ.snd < 1 + sizeOf axs := by
+        apply List.sizeOf_snd_lt_sizeOf_list hᵢ
+      exact @evaluates_subst axᵢ.snd request entities
+    exact @evaluates_subst_record axs request entities ih
+  | call xfn xs =>
+    have ih : ∀ xᵢ, xᵢ ∈ xs → EvaluatesSubst xᵢ request entities := by
+      intro xᵢ _
+      exact @evaluates_subst xᵢ request entities
+    exact @evaluates_subst_call xfn xs request entities ih
 
 theorem action_matches_env (env : Environment) (request : Request) (entities : Entities) :
-RequestAndEntitiesMatchEnvironment env request entities →
-request.action = env.reqty.action := by
-intro h₀
-simp [RequestAndEntitiesMatchEnvironment, InstanceOfRequestType] at h₀
-obtain ⟨ ⟨ _, h₁, _, _ ⟩ , _ , _⟩ := h₀
-assumption
+  RequestAndEntitiesMatchEnvironment env request entities →
+  request.action = env.reqty.action
+:= by
+  intro h₀
+  simp only [RequestAndEntitiesMatchEnvironment, InstanceOfRequestType] at h₀
+  obtain ⟨ ⟨ _, h₁, _, _ ⟩ , _ , _⟩ := h₀
+  exact h₁
 
 theorem typecheck_policy_is_sound (policy : Policy) (env : Environment) (t : CedarType) (request : Request) (entities : Entities) :
-RequestAndEntitiesMatchEnvironment env request entities →
-typecheckPolicy policy env = .ok t →
-∃ b : Bool, EvaluatesTo policy.toExpr request entities b := by
-intro h₁ h₂
-simp [typecheckPolicy] at h₂
-cases h₃ : typeOf (substituteAction env.reqty.action policy.toExpr) [] env <;> simp [h₃] at h₂
-split at h₂ <;> simp only [Except.ok.injEq] at h₂
-rename_i cp ht
-have hc := empty_capabilities_invariant request entities
-have ⟨_, v, h₄, h₅⟩ := type_of_is_sound hc h₁ h₃
-have ⟨b, h₆⟩ := instance_of_type_bool_is_bool v cp.fst h₅ ht
-subst h₆
-exists b
-simp [EvaluatesTo] at *
-cases h₄ with
-| inl h₁ =>
-  left
-  rw [← evaluates_subst policy.toExpr request entities]
-  rw [action_matches_env]
-  repeat assumption
-| inr h₁ => cases h₁ with
-  | inl h₂ =>
-    right
+  RequestAndEntitiesMatchEnvironment env request entities →
+  typecheckPolicy policy env = .ok t →
+  ∃ b : Bool, EvaluatesTo policy.toExpr request entities b
+:= by
+  intro h₁ h₂
+  simp only [typecheckPolicy] at h₂
+  cases h₃ : typeOf (substituteAction env.reqty.action policy.toExpr) [] env <;> simp only [List.empty_eq,
+    h₃] at h₂
+  split at h₂ <;> simp only [Except.ok.injEq] at h₂
+  rename_i cp ht
+  have hc := empty_capabilities_invariant request entities
+  have ⟨_, v, h₄, h₅⟩ := type_of_is_sound hc h₁ h₃
+  have ⟨b, h₆⟩ := instance_of_type_bool_is_bool v cp.fst h₅ ht
+  subst h₆
+  exists b
+  simp only [EvaluatesTo] at *
+  cases h₄ with
+  | inl h₁ =>
     left
     rw [← evaluates_subst policy.toExpr request entities]
     rw [action_matches_env]
     repeat assumption
-  | inr h₂ => cases h₂ with
-    | inl h₃ =>
-      right
+  | inr h₁ => cases h₁ with
+    | inl h₂ =>
       right
       left
       rw [← evaluates_subst policy.toExpr request entities]
       rw [action_matches_env]
       repeat assumption
-    | inr h₃ =>
-      right
-      right
-      right
-      rw [← evaluates_subst policy.toExpr request entities]
-      rw [action_matches_env]
-      repeat assumption
+    | inr h₂ => cases h₂ with
+      | inl h₃ =>
+        right
+        right
+        left
+        rw [← evaluates_subst policy.toExpr request entities]
+        rw [action_matches_env]
+        repeat assumption
+      | inr h₃ =>
+        right
+        right
+        right
+        rw [← evaluates_subst policy.toExpr request entities]
+        rw [action_matches_env]
+        repeat assumption
 
 theorem typecheck_policy_with_environments_is_sound (policy : Policy) (envs : List Environment) (request : Request) (entities : Entities) :
-(∀ env : Environment, env ∈ envs →
-RequestAndEntitiesMatchEnvironment env request entities) →
-typecheckPolicyWithEnvironments policy envs = .ok () →
-∃ b : Bool, EvaluatesTo policy.toExpr request entities b := by
-intro h₀ h₂
-simp [typecheckPolicyWithEnvironments] at h₂
-cases h₃ : List.mapM (typecheckPolicy policy) envs with
-| error => simp [h₃] at h₂
-| ok ts =>
-  simp [h₃] at h₂
-  cases h₄ : envs with
-  | nil =>
-    simp [h₄, pure, Except.pure] at h₃
-    subst h₃
-    simp [allFalse] at h₂
-  | cons h t =>
-      rw [List.mapM_ok_iff_forall₂] at h₃
-      have h₆ : RequestAndEntitiesMatchEnvironment h request entities := by
-        have h₇ : h ∈ envs := by simp [h₄]
-        specialize h₀ h
-        apply h₀ h₇
-      subst h₄
-      rw [List.forall₂_cons_left_iff] at h₃
-      simp only [exists_and_left] at h₃
-      obtain ⟨ b, _, _, _, _ ⟩ := h₃
-      apply typecheck_policy_is_sound policy h b
-      repeat assumption
+  (∀ env ∈ envs, RequestAndEntitiesMatchEnvironment env request entities) →
+  typecheckPolicyWithEnvironments policy envs = .ok () →
+  ∃ b : Bool, EvaluatesTo policy.toExpr request entities b
+:= by
+  intro h₀ h₂
+  simp only [typecheckPolicyWithEnvironments] at h₂
+  cases h₃ : List.mapM (typecheckPolicy policy) envs with
+  | error => simp only [h₃, Except.bind_err] at h₂
+  | ok ts =>
+    simp only [h₃, Except.bind_ok, ite_eq_right_iff, imp_false, Bool.not_eq_true] at h₂
+    cases h₄ : envs with
+    | nil =>
+      simp only [h₄, List.mapM_nil, pure, Except.pure, Except.ok.injEq] at h₃
+      subst h₃
+      simp only [allFalse, List.all_nil, Bool.true_eq_false] at h₂
+    | cons h t =>
+        rw [List.mapM_ok_iff_forall₂] at h₃
+        have h₆ : RequestAndEntitiesMatchEnvironment h request entities := by
+          have h₇ : h ∈ envs := by simp only [h₄, List.mem_cons, true_or]
+          specialize h₀ h
+          apply h₀ h₇
+        subst h₄
+        rw [List.forall₂_cons_left_iff] at h₃
+        simp only [exists_and_left] at h₃
+        obtain ⟨ b, _, _, _, _ ⟩ := h₃
+        apply typecheck_policy_is_sound policy h b
+        repeat assumption
 
 end Cedar.Thm
