cedar-lean/Cedar/Thm/Data/List/Lemmas.lean
@@ -1146,6 +1146,72 @@ theorem f_implies_g_then_subset {f g : α → Option β} {xs : List α} :
   apply And.intro h₂
   exact h₁ a b h₃
 
+/-! ### forM and mapM -/
+
+theorem mapM_forM {α β : Type} (f : α → Except β PUnit) (xs : List α) (ys : List PUnit) :
+  xs.mapM f = Except.ok ys → xs.forM f = Except.ok ()
+:= by
+  intro h₀
+  induction xs generalizing ys with
+  | nil => simp only [forM_nil', pure, Except.pure]
+  | cons xh xt ih =>
+    simp only [forM_cons']
+    cases h₁ : f xh with
+    | error =>
+      simp only [List.mapM_cons] at h₀
+      rw [h₁] at h₀
+      simp only [Except.bind_err] at h₀
+    | ok =>
+        simp only [List.mapM_cons, pure, Except.pure] at h₀
+        cases h₁ : f xh <;>
+        simp only [h₁, Except.bind_err, Except.bind_ok] at h₀
+        rename_i yh
+        cases h₂ : List.mapM f xt <;>
+        simp only [h₂, Except.bind_err, Except.bind_ok] at h₀
+        rename_i yt
+        simp only [Except.ok.injEq] at h₀
+        subst h₀
+        simp only [Except.bind_ok]
+        apply ih yt
+        assumption
+
+theorem forM_mapM {α β : Type} (f : α → Except β PUnit) (xs : List α) :
+  xs.forM f = Except.ok () → ∃ ys, xs.mapM f = Except.ok ys
+:= by
+  intro h₁
+  rw [← List.mapM'_eq_mapM]
+  induction xs
+  case nil =>
+    simp only [List.mapM'_nil, pure, Except.pure, Except.ok.injEq]
+    exists []
+  case cons xh xt ih =>
+    cases h₂ : f xh with
+    | error =>
+      simp only [List.mapM'_cons, pure, Except.pure]
+      simp only [forM_cons'] at h₁
+      rw [h₂] at h₁
+      simp only [Except.bind_err] at h₁
+    | ok y' =>
+      simp only [List.forM_cons'] at h₁
+      rw [h₂] at h₁
+      simp only [Except.bind_ok] at h₁
+      simp only [List.mapM'_cons, pure, Except.pure]
+      rw [h₂]
+      obtain ⟨ys, h₃⟩ := ih h₁
+      rw [h₃]
+      simp only [Except.bind_ok]
+      exists (y' :: ys)
+
+
+theorem forM_implies_all_ok {α β : Type} (xs : List α) (f : α → Except β Unit) :
+  xs.forM f = Except.ok () → (∀ x ∈ xs, f x = Except.ok ())
+:= by
+  intro h₀ x xin
+  obtain ⟨ys, h₁⟩ := forM_mapM f xs h₀
+  have h₂ := List.mapM_ok_implies_all_ok h₁ x
+  obtain ⟨_, _, h₅⟩ := h₂ xin
+  exact h₅
+
 /-! ### removeAll -/
 
 theorem removeAll_singleton_cons_of_neq [DecidableEq α] (x y : α) (xs : List α) :
@@ -1202,16 +1268,3 @@ theorem length_removeAll_le {α : Type u_1} [BEq α] (xs ys : List α) :
   omega
 
 end List
-
--- forM and mapM
-
-theorem forM_mapM {α β : Type} (f : α → Except β PUnit) (xs : List α) (ys : List PUnit) :
-xs.mapM f = Except.ok ys → xs.forM f = Except.ok () := by
-intro h₀
-rw [List.mapM_ok_iff_forall₂] at h₀
-sorry
-
-theorem forM_implies_all_ok {α β : Type} (xs : List α) (f : α → Except β Unit) : xs.forM f = Except.ok () →
-(∀ x ∈ xs, f x = Except.ok ()) := by
-intro h₀ x xin
-sorry
