cedar-lean/Cedar/Thm/Validation.lean
@@ -1,7 +1,30 @@
+/-
+ Copyright 2022-2023 Amazon.com, Inc. or its affiliates. All Rights Reserved.
+
+ Licensed under the Apache License, Version 2.0 (the "License");
+ you may not use this file except in compliance with the License.
+ You may obtain a copy of the License at
+
+      https://www.apache.org/licenses/LICENSE-2.0
+
+ Unless required by applicable law or agreed to in writing, software
+ distributed under the License is distributed on an "AS IS" BASIS,
+ WITHOUT WARRANTIES OR CONDITIONS OF ANY KIND, either express or implied.
+ See the License for the specific language governing permissions and
+ limitations under the License.
+-/
+
 import Cedar.Spec
 import Cedar.Data
 import Cedar.Validation
 import Cedar.Thm.Validation.Validator
+
+/-!
+This file contains the top-level correctness properties for the Cedar validator.
+We show that if validation succeeds, then for any request consistent with the schema,
+evaluation of every policy is "correct", that is, it either produces a boolean value,
+or throws one of the errors in the set of valid errors.
+--/
 
 namespace Cedar.Thm
 
@@ -10,37 +33,38 @@ open Cedar.Spec
 open Cedar.Validation
 
 /--
-If validation succeeds, then for any request consistent with the schema, either
-(1) evaluation of every policy produces a boolean or (2) returns an error TODO
+If a set of policies is well-typed (valid) with respect to the schema according to the validator,
+and the input request and entities are consistent with the schema, then every policy "evaluates correctly":
+this means that evaluation either produces a boolean value, or throws an error of type
+`entityDoesNotExist`, `extensionError`, or `arithBoundsError`. These errors cannot be protected against at
+validation time, as they depend on runtime information. 
 -/
 theorem validation_is_sound (policies : Policies) (schema : Schema) (request : Request) (entities : Entities) :
-validate policies schema = .ok () →
-(∀ env ∈ schema.toEnvironments,
-RequestAndEntitiesMatchEnvironment env request entities) →
-AllEvaluateCorrectly policies request entities := by
-intro h₀ h₁
-unfold validate at h₀
-simp [AllEvaluateCorrectly]
-cases h₃ : policies with
-| nil => simp [h₃]
-| cons h' t' =>
-  intro policy pin
-  simp [OneEvaluatesCorrectly]
-  apply typecheck_policy_with_environments_is_sound policy schema.toEnvironments request entities h₁
-  subst h₃
-  simp [List.forM_cons] at h₀
-  cases h₄ : (typecheckPolicyWithEnvironments h' schema.toEnvironments) <;> simp [h₄] at h₀
-  case ok _ =>
-    rw [List.mem_cons] at pin
-    cases pin with
-    | inl h₅ =>
-      subst h₅
-      assumption
-    | inr h₅ =>
-    apply forM_implies_all_ok t' (fun x => typecheckPolicyWithEnvironments x schema.toEnvironments)
-    repeat assumption
+  validate policies schema = .ok () →
+  RequestAndEntitiesMatchSchema schema request entities →
+  AllEvaluateCorrectly policies request entities
+:= by
+  intro h₀ h₁
+  unfold validate at h₀
+  simp only [AllEvaluateCorrectly]
+  cases h₃ : policies with
+  | nil => simp only [List.not_mem_nil, false_implies, implies_true]
+  | cons h' t' =>
+    intro policy pin
+    simp only [OneEvaluatesCorrectly]
+    apply typecheck_policy_with_environments_is_sound policy schema.toEnvironments request entities h₁
+    subst h₃
+    simp only [List.forM_cons'] at h₀
+    cases h₄ : (typecheckPolicyWithEnvironments h' schema.toEnvironments) <;> simp only [h₄,
+      Except.bind_err] at h₀
+    case ok _ =>
+      rw [List.mem_cons] at pin
+      cases pin with
+      | inl h₅ =>
+        subst h₅
+        assumption
+      | inr h₅ =>
+      apply List.forM_implies_all_ok t' (fun x => typecheckPolicyWithEnvironments x schema.toEnvironments)
+      repeat assumption
 
-
-
-
--- end Cedar.Thm
+end Cedar.Thm
